

## Lec 6

29 January 2026 08:01

 $X(K) \rightarrow M$  subspace $x, y \in X$  $x \sim y \Leftrightarrow x - y \in M$  $\sim$  is an equivalence relation

$$[x] = x + M$$

$$X/M = \{[x] \mid x \in X\} = \{x + M \mid x \in X\}$$

 $+$ ,  $\cdot$  well defined

$$(x + M) + (y + M) = (x + y) + M$$

$$\|x + M\| = \text{dis}(x, M) \quad \left( \text{dis}(x, M) = 0 \Leftrightarrow x \in \overline{M} \right)$$

$$M \subseteq \overline{X} \quad \text{closed}$$

 $\|\cdot\|$  on  $X/M$ Theorem

let  $X$  be a Banach space and  $M$  be a closed subspace of  $X$ .  
Then  $X/M$  is a Banach space.

Lemma let  $(y_n)$  is a CS in NLSYthen  $\exists$  a subseq  $(y_{n_k})$  of  $(y_n)$  st

$$\|y_{n_{k+1}} - y_{n_k}\| < 2^{-k}$$

proof

$$\|x_m - x_n\| < \frac{1}{2^{-n}} \quad \forall m, n > n_k$$

$$n_1 < n_2 < n_3 < \dots$$

 $\hookrightarrow$  subseqGiven  $(y_n)$  is CSby def.  $\forall \varepsilon > 0 \exists N$  such that

$$\|y_m - y_n\| < \varepsilon \quad \forall n, m \geq N$$

choose

$$\varepsilon = 1/2 \quad \text{then}$$

$$\varepsilon = 1/2^2$$

 $\vdots$ 

get sub seq

Claim:  $X/M$  is a BS $M$ : closedlet  $x_n + M$  be a CS in  $X/M$ 

when a CS have a convergent subseq then the CS is also convergent

to show  $\exists x_{n_k}$  st  $x_{n_k} + M$  is convergent $X/M$  is a nls so for  $(x_n + M) \exists$  a subseq $(x_{n_k} + M)$  such that

$$\|(x_{n_k} + M) - (x_{n_l} + M)\| < 1/2^{-k} \quad \square$$

consider  $y_1 = 0$

$$\inf_{y \in M} \| (x_{n_1} - y_1) - (x_{n_2} - y) \| = \inf_{y \in M} \| (x_{n_1} - x_{n_2}) + y \|$$

$$\Rightarrow \| x_{n_1} - x_{n_2} + M \| < \frac{1}{2}$$

$\exists y_2$  such that

$$\| (x_{n_1} - y_1) - (x_{n_2} - y_2) \| < 2 \cdot \frac{1}{2}$$

(using def<sup>n</sup> of infimum)

since  $y_2 \in M$

$$\inf_{y \in M} \| (x_{n_2} - y_2) - (x_{n_3} - y) \| = \inf_{y \in M} \| (x_{n_2} - x_{n_3}) + y \|^2$$

$$( \text{dist}(x, M) = \text{dist}(x+y, M) \quad y \in M )$$

$$= \| x_{n_2} - x_{n_3} + M \|$$

$$< \frac{1}{2}^2$$

By def. of inf.  $\exists y_3 \in M$  such that

$$\| (x_{n_2} - y_2) - (x_{n_3} - y_3) \| < 2 \cdot \frac{1}{2^2}$$

continuing like this  $\exists y_k$  such that

$$\| (x_{n_k} - y_k) - (x_{n_{k+1}} - y_{k+1}) \| < 2 \cdot \frac{1}{2^k}$$

$$z_k = x_{n_k} - y_k$$

$$\text{we can say } \| z_k - z_{k+1} \| < \frac{1}{2^{k-1}}$$

if a seq satisfy this  
then that is a cauchy convergent seq

$$z_k \rightarrow z \quad (z \in X) \quad \text{as } X \text{ is B.S.}$$

$$\| (x_{n_k} + m) - (z + m) \| = \| (x_{n_k} - z) + m \|^2$$

$$= \| x_{n_k} - y_k - z + m \|^2$$

$$= \| z_k - z + m \|^2$$

$$( = \inf \| z_k - z + u \|, \quad u \in M )$$

$$\leq \| z_k - z \| \rightarrow 0 \quad \text{as } k \rightarrow \infty$$

$$\therefore (x_{n_k} + m) \rightarrow (z + m) \quad \text{as } k \rightarrow \infty$$

Converse

theorem let  $X$  be a NLS and  $M$  a closed subspace

$\mathcal{U}_X$

If  $X/M$  is BS and  $M$  is also BS  
then  $X$  is BS

proof: let  $(x_n)$  be a CS in  $X$

$$\text{then } \|(x_n + M) - (x_m + M)\| = \|x_n - x_m + M\|$$

$$= \inf \{ \|x_n - x_m + u\| : u \in M \}$$

as  $0 \in M$

$$\leq \|x_n - x_m\| \rightarrow 0 \quad \text{as } m, n \rightarrow \infty$$

$\therefore (x_n + M)$  is CS in  $X/M$

since  $X/M$  is BS

then  $x_n + M \rightarrow x + M \quad x \in X$

$$\|(x_n + M) - (x + M)\| < \varepsilon \quad \forall n \geq N_0$$

$$\Rightarrow \|x_n - x + M\| < \varepsilon \quad \forall n \geq N_0$$

$$\text{LHS} = \inf \{ \|x_n - x + y\| : y \in M \}$$

choose  $y_n \in M$  s.t.

$$\|x_n - x + y_n\| < \|x_n - x + M\| + \frac{1}{n}$$

$$\rightarrow 0 \quad \text{as } n \rightarrow \infty$$

$\therefore x_n + y_n \rightarrow x$  in  $X$

now to show  $(y_n)$  is a CS (H.W.)

$$\|y_n - y_m\| = \|y_n + x_n - x_n + x_m - x_m - y_m\|$$

## Convergent series in NLS

let  $(x_n)$  be a seq in a NLS  $X$ .

consider  $\sum_{n \in \mathbb{N}} x_n$

this series convergent to  $x$

$$S_N = \sum_{n=1}^N x_n \rightarrow x \quad \text{in } X$$

$$\text{means } \|S_N - x\|_X \rightarrow 0 \quad \text{as } N \rightarrow \infty$$

## Absolutely convergent series

If  $\sum \|x_n\| < \infty$  then  $\sum x_n$  is absolute convergent

Ex in  $\mathbb{R}$   $\sum_{n=1}^{\infty} (-1)^{n+1} \frac{1}{n} \rightarrow \text{convergent}$

but  $\sum_{n=1}^{\infty} \left| (-1)^{n+1} \frac{1}{n} \right| = \sum_{n=1}^{\infty} \frac{1}{n}$  is not convergent

### Remark

[absolute convergent in a NLS is NOT stronger than convergence]

Ex

$X = \mathcal{P}([0, 1])$ ,  $\|\cdot\|_{\infty}$

$$\sum_{n=1}^{\infty} \frac{x^n}{n!}$$

here  $\sum_{n=1}^{\infty} \left\| \frac{x^n}{n!} \right\|$  is convergent

$\therefore \sum \frac{x^n}{n!}$  is absolutely convergent

however  $\sum \frac{x^n}{n!} \rightarrow e^x \notin \mathcal{P}([0, 1])$

} Not convergent

### Theorem

for a NLS  $X$

$X$  is BS  $\Leftrightarrow$  every abs. convergent series in  $X$  is convergent

proof: Suppose  $X$  is a BS  
let  $\sum x_n$  be abs convergent  
(i.e.  $\sum \|x_n\|$  is convergent)

let  $S_N = \sum_{n=1}^N x_n$   $N > M$

$$\|S_N - S_M\| = \left\| \sum_{n=1}^N x_n - \sum_{n=1}^M x_n \right\| \leq \sum_{n=M+1}^N \|x_n\|$$

Since  $X$  is BS

so  $S_N$  is convergent and that

implies  $\sum x_n$  is convergent.

